Test/civl/alloc.bpl
@@ -3,173 +3,203 @@
 function {:builtin "MapConst"} MapConstBool(bool) : [int]bool;
 
 type lmap;
-function {:linear "mem"} dom(lmap): [int]bool;
-function map(lmap): [int]int;
+function {:linear "mem"} dom(lmap) : [int]bool;
+function map(lmap) : [int]int;
 function cons([int]bool, [int]int) : lmap;
-axiom (forall x: [int]bool, y: [int]int :: {cons(x,y)} dom(cons(x, y)) == x && map(cons(x,y)) == y);
+axiom (forall x:[int]bool, y:[int]int :: {cons(x,y)} dom(cons(x, y)) == x && map(cons(x,y)) == y);
+axiom (forall x: lmap :: {dom(x)} {map(x)} cons(dom(x), map(x)) == x);
 
-function EmptyLmap(): (lmap);
-axiom (dom(EmptyLmap()) == MapConstBool(false));
+function Empty(m:[int]int) : lmap;
+axiom (forall m: [int]int :: Empty(m) == cons(MapConstBool(false), m));
 
-function Add(x: lmap, i: int): (lmap);
-axiom (forall x: lmap, i: int :: dom(Add(x, i)) == dom(x)[i:=true] && map(Add(x, i)) == map(x));
+function Add(x:lmap, i:int): lmap;
+axiom (forall x:lmap, i:int :: dom(Add(x, i)) == dom(x)[i:=true] && map(Add(x, i)) == map(x));
 
-function Remove(x: lmap, i: int): (lmap);
-axiom (forall x: lmap, i: int :: dom(Remove(x, i)) == dom(x)[i:=false] && map(Remove(x, i)) == map(x));
+function Remove(x:lmap, i:int): lmap;
+axiom (forall x:lmap, i:int :: dom(Remove(x, i)) == dom(x)[i:=false] && map(Remove(x, i)) == map(x));
 
-function {:inline} PoolInv(unallocated:[int]bool, pool: lmap) : (bool)
+function {:inline} PoolInv(unallocated:[int]bool, pool:lmap) : (bool)
 {
-    (forall x: int :: unallocated[x] ==> dom(pool)[x])
+  (forall x:int :: unallocated[x] ==> dom(pool)[x])
 }
 
-procedure {:yields} {:layer 2} Main()
+procedure {:yields} {:layer 2} Main ()
 requires {:layer 1} PoolInv(unallocated, pool);
 ensures  {:layer 1} PoolInv(unallocated, pool);
 {
-   var {:layer 1} {:linear "mem"} l: lmap;
-   var i: int;
-   par Yield() | Dummy();
-   while (*)
-   invariant {:layer 1} PoolInv(unallocated, pool);
-   {
-      call  l, i := Alloc();
-      async call Thread(l, i);
-      par Yield() | Dummy();
-   }
-   par Yield() | Dummy();
+  var {:layer 1} {:linear "mem"} l:lmap;
+  var i:int;
+  par Yield() | Dummy();
+  while (*)
+  invariant {:layer 1} PoolInv(unallocated, pool);
+  {
+    call  l, i := Alloc();
+    async call Thread(l, i);
+    par Yield() | Dummy();
+  }
+  par Yield() | Dummy();
 }
 
-procedure {:yields} {:layer 2} Thread({:layer 1} {:linear_in "mem"} local_in: lmap, i: int)
+procedure {:yields} {:layer 2} Thread ({:layer 1} {:linear_in "mem"} local_in:lmap, i:int)
 requires {:layer 1} PoolInv(unallocated, pool);
 ensures  {:layer 1} PoolInv(unallocated, pool);
 requires {:layer 1} dom(local_in)[i] && map(local_in)[i] == mem[i];
 requires {:layer 2} dom(local_in)[i];
 {
-    var y, o: int;
-    var {:layer 1} {:linear "mem"} local: lmap;
-    var {:layer 1} {:linear "mem"} l: lmap;
+  var y, o:int;
+  var {:layer 1} {:linear "mem"} local:lmap;
+  var {:layer 1} {:linear "mem"} l:lmap;
 
-    par YieldMem(local_in, i) | Dummy();
-    call local := Copy(local_in);
-    call local := Write(local, i, 42);
-    call o := Read(local, i);
+  par YieldMem(local_in, i) | Dummy();
+  call local := Write(local_in, i, 42);
+  call o := Read(local, i);
+  assert {:layer 2} o == 42;
+  while (*)
+  invariant {:layer 1} PoolInv(unallocated, pool);
+  {
+    call l, y := Alloc();
+    call l := Write(l, y, 42);
+    call o := Read(l, y);
     assert {:layer 2} o == 42;
-    while (*)
-    invariant {:layer 1} PoolInv(unallocated, pool);
-    {
-        call l, y := Alloc();
-        call l := Write(l, y, 42);
-        call o := Read(l, y);
-        assert {:layer 2} o == 42;
-        call Free(l, y);
-        par Yield() | Dummy();
-    }
+    call Free(l, y);
     par Yield() | Dummy();
+  }
+  par Yield() | Dummy();
 }
 
-procedure {:pure} {:inline 1} Copy({:linear_in "mem"} l: lmap) returns ({:linear "mem"} l': lmap)
+procedure {:right} {:layer 2} atomic_Alloc() returns ({:linear "mem"} l:lmap, i:int)
+modifies pool;
 {
-    l' := l;
+  var m:[int]int;
+  assume dom(pool)[i];
+  pool := Remove(pool, i);
+  l := Add(Empty(m), i);
 }
 
-procedure {:yields} {:layer 1,2} Alloc() returns ({:layer 1} {:linear "mem"} l: lmap, i: int)
+procedure {:yields} {:layer 1} {:refines "atomic_Alloc"} Alloc() returns ({:layer 1} {:linear "mem"} l:lmap, i:int)
 requires {:layer 1} PoolInv(unallocated, pool);
 ensures  {:layer 1} PoolInv(unallocated, pool);
 ensures  {:layer 1} dom(l)[i] && map(l)[i] == mem[i];
-ensures {:right} |{ A: assume dom(l)[i]; return true; }|;
 {
-    call Yield();
-    call i := PickAddr();
-    call l := AllocLinear(i);
-    call YieldMem(l, i);
+  call Yield();
+  call i := PickAddr();
+  call l := AllocLinear(i);
+  call YieldMem(l, i);
 }
 
-procedure {:yields} {:layer 1,2} Free({:layer 1} {:linear_in "mem"} l: lmap, i: int)
+procedure {:left} {:layer 2} atomic_Free({:linear_in "mem"} l:lmap, i:int)
+modifies pool;
+{
+  assert dom(l)[i];
+  pool := Add(pool, i);
+}
+
+procedure {:yields} {:layer 1} {:refines "atomic_Free"} Free({:layer 1} {:linear_in "mem"} l:lmap, i:int)
 requires {:layer 1} PoolInv(unallocated, pool);
 ensures  {:layer 1} PoolInv(unallocated, pool);
 requires {:layer 1} dom(l)[i];
-ensures {:both} |{ A: return true; }|;
 {
-    call Yield();
-    call FreeLinear(l, i);
-    call ReturnAddr(i);
-    call Yield();
+  call Yield();
+  call FreeLinear(l, i);
+  call ReturnAddr(i);
+  call Yield();
 }
 
-procedure {:yields} {:layer 1,2} Read({:layer 1} {:linear "mem"} l: lmap, i: int) returns (o: int)
+procedure {:both} {:layer 2} atomic_Read ({:linear "mem"} l:lmap, i:int) returns (o:int)
+{
+  assert dom(l)[i];
+  o := map(l)[i];
+}
+
+procedure {:both} {:layer 2} atomic_Write ({:linear_in "mem"} l:lmap, i:int, o:int) returns ({:linear "mem"} l':lmap)
+{
+  assert dom(l)[i];
+  l' := cons(dom(l), map(l)[i := o]);
+}
+
+procedure {:yields} {:layer 1} {:refines "atomic_Read"} Read ({:layer 1} {:linear "mem"} l:lmap, i:int) returns (o:int)
 requires {:layer 1} PoolInv(unallocated, pool);
 ensures  {:layer 1} PoolInv(unallocated, pool);
 requires {:layer 1} dom(l)[i] && map(l)[i] == mem[i];
-ensures {:both} |{ A: assert dom(l)[i]; o := map(l)[i]; return true; }|;
 {
-    call YieldMem(l, i);
-    call o := ReadLow(i);
-    call YieldMem(l, i);
+  call YieldMem(l, i);
+  call o := ReadLow(i);
+  call YieldMem(l, i);
 }
 
-procedure {:yields} {:layer 1,2} Write({:layer 1} {:linear_in "mem"} l: lmap, i: int, o: int) returns ({:layer 1} {:linear "mem"} l': lmap)
+procedure {:yields} {:layer 1} {:refines "atomic_Write"} Write ({:layer 1} {:linear_in "mem"} l:lmap, i:int, o:int) returns ({:layer 1} {:linear "mem"} l':lmap)
 requires {:layer 1} PoolInv(unallocated, pool);
 ensures  {:layer 1} PoolInv(unallocated, pool);
 requires {:layer 1} dom(l)[i] && map(l)[i] == mem[i];
 ensures  {:layer 1} dom(l')[i] && map(l')[i] == mem[i];
-ensures {:both} |{ A: assert dom(l)[i]; l' := cons(dom(l), map(l)[i := o]); return true; }|;
 {
-    call YieldMem(l, i);
-    call WriteLow(i, o);
-    call l' := WriteLinear(l, i, o);
-    call YieldMem(l', i);
+  call YieldMem(l, i);
+  call WriteLow(i, o);
+  call l' := WriteLinear(l, i, o);
+  call YieldMem(l', i);
 }
 
-procedure {:layer 1} AllocLinear(i: int) returns ({:linear "mem"} l: lmap);
+procedure {:layer 1} AllocLinear (i:int) returns ({:linear "mem"} l:lmap);
 modifies pool;
 requires dom(pool)[i];
-ensures pool == Remove(old(pool), i) && dom(l)[i] && map(l)[i] == mem[i];
+ensures  pool == Remove(old(pool), i) && l == Add(Empty(mem), i);
 
-procedure {:layer 1} FreeLinear({:linear_in "mem"} l: lmap, i: int);
+procedure {:layer 1} FreeLinear ({:linear_in "mem"} l:lmap, i:int);
 modifies pool;
 requires dom(l)[i];
-ensures pool == Add(old(pool), i);
+ensures  pool == Add(old(pool), i);
 
-procedure {:layer 1} WriteLinear({:layer 1} {:linear_in "mem"} l: lmap, i: int, o: int) returns ({:layer 1} {:linear "mem"} l': lmap);
+procedure {:layer 1} WriteLinear ({:layer 1} {:linear_in "mem"} l:lmap, i:int, o:int) returns ({:layer 1} {:linear "mem"} l':lmap);
 requires dom(l)[i];
-ensures l' == cons(dom(l), map(l)[i := o]);
+ensures  l' == cons(dom(l), map(l)[i := o]);
 
-procedure {:yields} {:layer 1} Yield()
+procedure {:yields} {:layer 1} Yield ()
 requires {:layer 1} PoolInv(unallocated, pool);
-ensures {:layer 1} PoolInv(unallocated, pool);
+ensures  {:layer 1} PoolInv(unallocated, pool);
 {
-    yield;
-    assert {:layer 1} PoolInv(unallocated, pool);
+  yield;
+  assert {:layer 1} PoolInv(unallocated, pool);
 }
 
-procedure {:yields} {:layer 1} YieldMem({:layer 1} {:linear "mem"} l: lmap, i: int)
+procedure {:yields} {:layer 1} YieldMem ({:layer 1} {:linear "mem"} l:lmap, i:int)
 requires {:layer 1} PoolInv(unallocated, pool);
 ensures  {:layer 1} PoolInv(unallocated, pool);
 requires {:layer 1} dom(l)[i] && map(l)[i] == mem[i];
-ensures {:layer 1} dom(l)[i] && map(l)[i] == mem[i];
+ensures  {:layer 1} dom(l)[i] && map(l)[i] == mem[i];
 {
-    yield;
-    assert {:layer 1} PoolInv(unallocated, pool);
-    assert {:layer 1} dom(l)[i] && map(l)[i] == mem[i];
+  yield;
+  assert {:layer 1} PoolInv(unallocated, pool);
+  assert {:layer 1} dom(l)[i] && map(l)[i] == mem[i];
 }
 
 procedure {:yields} {:layer 2} Dummy()
 {
-    yield;
+  yield;
 }
 
-var {:layer 1, 1} {:linear "mem"} pool: lmap;
+var {:layer 1, 2} {:linear "mem"} pool:lmap;
 var {:layer 0, 1} mem:[int]int;
 var {:layer 0, 1} unallocated:[int]bool;
 
-procedure {:yields} {:layer 0, 1} ReadLow(i: int) returns (o: int);
-ensures {:atomic} |{ A: o := mem[i]; return true; }|;
+procedure {:atomic} {:layer 1} atomic_ReadLow (i:int) returns (o:int)
+{ o := mem[i]; }
 
-procedure {:yields} {:layer 0, 1} WriteLow(i: int, o: int);
-ensures {:atomic} |{ A: mem[i] := o; return true; }|;
+procedure {:atomic} {:layer 1} atomic_WriteLow (i:int, o:int)
+modifies mem;
+{ mem[i] := o; }
 
-procedure {:yields} {:layer 0, 1} PickAddr() returns (i: int);
-ensures {:atomic} |{ A: assume unallocated[i]; unallocated[i] := false; return true; }|;
+procedure {:atomic} {:layer 1} atomic_PickAddr () returns (i:int)
+modifies unallocated;
+{
+  assume unallocated[i];
+  unallocated[i] := false;
+}
 
-procedure {:yields} {:layer 0, 1} ReturnAddr(i: int);
-ensures {:atomic} |{ A: unallocated[i] := true; return true; }|;
+procedure {:atomic} {:layer 1} atomic_ReturnAddr (i:int)
+modifies unallocated;
+{ unallocated[i] := true; }  
+
+procedure {:yields} {:layer 0} {:refines "atomic_ReadLow"} ReadLow (i:int) returns (o:int);
+procedure {:yields} {:layer 0} {:refines "atomic_WriteLow"} WriteLow (i:int, o:int);
+procedure {:yields} {:layer 0} {:refines "atomic_PickAddr"} PickAddr () returns (i:int);
+procedure {:yields} {:layer 0} {:refines "atomic_ReturnAddr"} ReturnAddr (i:int);
