Test/civl/chris.bpl
@@ -1,21 +1,21 @@
 // RUN: %boogie -noinfer -typeEncoding:m -useArrayTheory "%s" > "%t"
 // RUN: %diff "%s.expect" "%t"
-var{:layer 1} x:int;
+var{:layer 1,3} x:int;
 
 procedure{:yields}{:layer 2} Havoc()
-  ensures{:atomic} |{ A: return true; }|;
 {
   yield;
 }
 
-procedure{:yields}{:layer 1} Recover()
-  ensures{:atomic} |{ A: assert x == 5; return true; }|;
+procedure{:atomic}{:layer 2,3} AtomicRecover()
+{ assert x == 5; }
+
+procedure{:yields}{:layer 1} {:refines "AtomicRecover"} Recover()
 {
   yield;
 }
 
 procedure{:yields}{:layer 3} P()
-  ensures{:atomic} |{ A: return true; }|;
   requires{:layer 2,3} x == 5;
   ensures {:layer 2,3} x == 5;
 {
