Test/civl/chris3.bpl
@@ -1,17 +1,19 @@
 // RUN: %boogie -noinfer -typeEncoding:m -useArrayTheory "%s" > "%t"
 // RUN: %diff "%s.expect" "%t"
-procedure{:yields}{:layer 94,94} H()
+
+procedure{:atomic}{:layer 95} skip() { }
+
+procedure{:yields}{:layer 94} {:refines "skip"} H()
+{
+  yield;
+}
+  
+procedure{:yields}{:layer 94} {:refines "skip"} A()
 {
   yield;
 }
 
-procedure{:yields}{:layer 94,95} A()
-  ensures{:atomic} |{ A: return true; }|;
-{
-  yield;
-}
-
-procedure{:yields}{:layer 95,95} P()
+procedure{:yields}{:layer 95} P()
 {
   yield;
   par A() | H();
