Test/civl/chris4.bpl
@@ -1,13 +1,13 @@
 // RUN: %boogie -noinfer -typeEncoding:m -useArrayTheory "%s" > "%t"
 // RUN: %diff "%s.expect" "%t"
-procedure{:yields}{:layer 94,95} Test()
+procedure{:yields}{:layer 94} Test()
 {
   yield;
   L:
   yield;
 }
 
-procedure{:yields}{:layer 94,95} Test2()
+procedure{:yields}{:layer 94} Test2()
 {
   yield;
   assert{:layer 94} 2 + 2 == 3;
