Test/civl/chris6.bpl
@@ -1,11 +1,11 @@
 // RUN: %boogie -noinfer -useArrayTheory "%s" > "%t"
 // RUN: %diff "%s.expect" "%t"
-procedure{:extern}{:yields}{:layer 1,2} P1();
-  requires{:layer 1} false;
-  ensures{:atomic} |{ A: return true; }|;
+procedure{:atomic}{:layer 2} atomic_P1() { }
 
-procedure{:yields}{:layer 2,3} P2()
-  ensures{:atomic} |{ A: return true; }|;
+procedure{:yields}{:layer 1} {:refines "atomic_P1"} P1();
+  requires{:layer 1} false;
+
+procedure{:yields}{:layer 2} P2()
 {
   assert{:layer 1} false;
   yield;
