Test/civl/chris8.bpl
@@ -2,11 +2,10 @@
 // RUN: %diff "%s.expect" "%t"
 var{:layer 1,1} x:int;
 
-procedure{:layer 1}{:extern} P1(i:int);
-procedure{:pure}{:extern} P2(j:int);
+procedure{:layer 1} P1(i:int);
+procedure P2(j:int);
 
-procedure{:yields}{:layer 1,2} A1({:layer 1}i:int)
-  ensures {:atomic} |{ A: return true; }|;
+procedure{:yields}{:layer 1} A1({:layer 1}i:int)
 {
   yield;
   call P1(i);
