Test/civl/linearity-bug-2.bpl
@@ -7,14 +7,13 @@
 
 var {:linear "lin"} {:layer 1,2} set : [int]bool;
 
-procedure {:yields} {:layer 1,2} foo ({:linear "lin"} i : int);
-ensures {:atomic} |{
- A: set[i] := true;
-    return true;
-}|;
+procedure {:atomic} {:layer 2} atomic_foo ({:linear "lin"} i : int)
+modifies set;
+{ set[i] := true; }
+
+procedure {:yields} {:layer 1} {:refines "atomic_foo"} foo ({:linear "lin"} i : int);
 
 procedure {:yields} {:layer 2} main ({:linear "lin"} i : int)
-ensures {:atomic} |{ A: return true; }|;
 {
   yield;
   call foo(i);
