Test/civl/lock2.bpl
@@ -26,8 +26,11 @@ procedure {:yields} {:layer 2} Customer()
     yield;
 }
 
-procedure {:yields} {:layer 1,2} Enter()
-ensures {:atomic} |{ A: assume b == 0; b := 1; return true; }|;
+procedure {:atomic} {:layer 2} AtomicEnter()
+modifies b;
+{ assume b == 0; b := 1; }
+
+procedure {:yields} {:layer 1} {:refines "AtomicEnter"} Enter()
 {
     var _old, curr: int;
     yield;
@@ -49,15 +52,24 @@ ensures {:atomic} |{ A: assume b == 0; b := 1; return true; }|;
     yield;
 }
 
-procedure {:yields} {:layer 0,2} Read() returns (val: int);
-ensures {:atomic} |{ A: val := b; return true; }|;
+procedure {:atomic} {:layer 1,2} AtomicRead() returns (val: int)
+{ val := b; }
 
-procedure {:yields} {:layer 0,2} CAS(prev: int, next: int) returns (_old: int);
-ensures {:atomic} |{
-A: _old := b; goto B, C;
-B: assume _old == prev; b := next; return true;
-C: assume _old != prev; return true;
-}|;
+procedure {:yields} {:layer 0} {:refines "AtomicRead"} Read() returns (val: int);
 
-procedure {:yields} {:layer 0,2} Leave();
-ensures {:atomic} |{ A: b := 0; return true; }|;
+procedure {:atomic} {:layer 1,2} AtomicCAS(prev: int, next: int) returns (_old: int)
+modifies b;
+{
+  _old := b;
+  if (_old == prev) {
+    b := next;
+  }
+}
+
+procedure {:yields} {:layer 0} {:refines "AtomicCAS"} CAS(prev: int, next: int) returns (_old: int);
+
+procedure {:atomic} {:layer 1,2} AtomicLeave()
+modifies b;
+{ b := 0; }
+
+procedure {:yields} {:layer 0} {:refines "AtomicLeave"} Leave();
