Test/civl/par-incr.bpl
@@ -1,13 +1,19 @@
 // RUN: %boogie -noinfer -typeEncoding:m -useArrayTheory "%s" > "%t"
 // RUN: %diff "%s.expect" "%t"
 
-var {:layer 0} x: int;
+var {:layer 0,3} x: int;
 
-procedure {:yields} {:layer 0,1} Incr();
-ensures {:right} |{ A: x := x + 1; return true; }|;
+procedure {:right} {:layer 1} AtomicIncr()
+modifies x;
+{ x := x + 1; }
 
-procedure {:yields} {:layer 1,2} Incr2()
-ensures {:right} |{ A: x := x + 2; return true; }|;
+procedure {:yields} {:layer 0} {:refines "AtomicIncr"} Incr();
+
+procedure {:right} {:layer 2} AtomicIncr2()
+modifies x;
+{ x := x + 2; }
+
+procedure {:yields} {:layer 1} {:refines "AtomicIncr2"} Incr2()
 {
   yield;
   par Incr() | Incr();
@@ -19,8 +25,11 @@ procedure {:yields} {:layer 1} Yield()
    yield;
 }
 
-procedure {:yields} {:layer 2,3} Incr4()
-ensures {:atomic} |{ A: x := x + 4; return true; }|;
+procedure {:atomic} {:layer 3} AtomicIncr4()
+modifies x;
+{ x := x + 4; }
+
+procedure {:yields} {:layer 2} {:refines "AtomicIncr4"} Incr4()
 {
   yield;
   par Incr2() | Incr2() | Yield();
