Test/civl/t1.bpl
@@ -21,11 +21,17 @@ function {:inline} {:linear "2"} SetCollector2(x: [int]bool) : [int]bool
 var {:layer 0,1} g: int;
 var {:layer 0,1} h: int;
 
-procedure {:yields} {:layer 0,1} SetG(val:int);
-ensures {:atomic} |{A: g := val; return true; }|;
+procedure {:atomic} {:layer 1} AtomicSetG(val:int)
+modifies g;
+{ g := val; }
 
-procedure {:yields} {:layer 0,1} SetH(val:int);
-ensures {:atomic} |{A: h := val; return true; }|;
+procedure {:yields} {:layer 0} {:refines "AtomicSetG"} SetG(val:int);
+
+procedure {:atomic} {:layer 1} AtomicSetH(val:int)
+modifies h;
+{ h := val; }
+
+procedure {:yields} {:layer 0} {:refines "AtomicSetH"} SetH(val:int);
 
 procedure {:yields} {:layer 1} Yield({:linear "1"} x: [int]bool)
 requires {:layer 1} x == mapconstbool(true) && g == 0;
@@ -43,8 +49,10 @@ ensures {:layer 1} xl != 0;
     yield;
 }
 
-procedure {:yields} {:layer 0,1} AllocateLow() returns ({:linear "tid"} xls: int);
-ensures {:atomic} |{ A: assume xls != 0; return true; }|;
+procedure {:atomic} {:layer 1} AtomicAllocateLow() returns ({:linear "tid"} xls: int)
+{ assume xls != 0; }
+
+procedure {:yields} {:layer 0} {:refines "AtomicAllocateLow"} AllocateLow() returns ({:linear "tid"} xls: int);
 
 procedure {:yields} {:layer 1} A({:linear_in "tid"} tid_in: int, {:linear_in "1"} x: [int]bool, {:linear_in "2"} y: [int]bool) returns ({:linear "tid"} tid_out: int)
 requires {:layer 1} x == mapconstbool(true);
